Library/DRandom.dfy
@@ -27,15 +27,22 @@ module {:extern "DafnyLibraries"} DafnyLibraries {
 
     method Uniform(n: nat) returns (u: nat)
       modifies this
+      decreases *
       requires 0 < n
       ensures UniformModel(n)(old(s)) == (u, s)
-      decreases *
 
     method UniformInterval(a: int, b: int) returns (u: int)
       modifies this
+      decreases *
       requires a < b
       ensures UniformIntervalModel(a, b)(old(s)) == (u, s)
+
+    method Geometric() returns (c: nat)
+      modifies this
       decreases *
+      ensures !old(s)(c)
+      ensures forall i | 0 <= i < c :: old(s)(i)
+      ensures s == IterateTail(old(s), c + 1)
 
     method Bernoulli(p: real) returns (c: bool) 
       modifies this
@@ -54,8 +61,8 @@ module {:extern "DafnyLibraries"} DafnyLibraries {
     // Based on https://arxiv.org/pdf/1304.1916.pdf; unverified.
     method Uniform(n: nat) returns (u: nat)
       modifies this
-      requires n > 0
       decreases *
+      requires n > 0
       ensures UniformModel(n)(old(s)) == (u, s)
     {
       assume {:axiom} false;
@@ -78,8 +85,8 @@ module {:extern "DafnyLibraries"} DafnyLibraries {
     
     method UniformInterval(a: int, b: int) returns (u: int)
       modifies this
-      requires a < b
       decreases *
+      requires a < b
       ensures UniformIntervalModel(a, b)(old(s)) == (u, s)
     {
       var v := Uniform(b - a);
@@ -87,6 +94,46 @@ module {:extern "DafnyLibraries"} DafnyLibraries {
       assert UniformIntervalModel(a, b)(old(s)) == (a + v, s);
       u := a + v;
     }
+
+    method Geometric() returns (c: nat)
+      modifies this
+      decreases *
+      ensures !old(s)(c)
+      ensures forall i | 0 <= i < c :: old(s)(i)
+      ensures s == IterateTail(old(s), c + 1)
+    {
+      c := 0;
+      var b := Coin();
+      assert old(s)(c) == b;
+      assert s == IterateTail(old(s), c + 1);
+      while b 
+        decreases *
+        invariant s == IterateTail(old(s), c + 1)
+        invariant b == IterateTail(old(s), c)(0)
+        invariant b == old(s)(c)
+        invariant forall i | 0 <= i < c :: old(s)(i)
+      {
+        var s' := s;
+        var c' := c;
+        var b' := b;
+        assert forall i | 0 <= i < c' :: old(s)(i);
+        assert s' == IterateTail(old(s), c' + 1);
+        assert b' == IterateTail(old(s), c')(0);
+        b := Coin();
+        assert (b, s) == (Head(s'), Tail(s'));
+        assert b == IterateTail(old(s), c' + 1)(0);
+        assert s == Tail(IterateTail(old(s), c' + 1));
+        TailOfIterateTail(old(s), c' + 1);
+        assert s == IterateTail(old(s), (c' + 1) + 1);
+        c := c + 1;
+        assert c == c' + 1;
+        assert old(s)(c') by {
+          assert b';
+        }
+        assert s == IterateTail(old(s), c + 1);
+        assert b == IterateTail(old(s), c)(0);
+      }
+    } 
 
     method Bernoulli(p: real) returns (c: bool)
       modifies this 
